ChoiceTyping/theories/ResultWorldFreshForall.v
@@ -44,212 +44,9 @@ Lemma FExprResultOn_dom_exact_domain_eq_let_result_world_on
   n ⊨ FExprResultOn (dom Σ) e ν →
   n = let_result_world_on e ν m Hfresh Hresult.
 Proof.
-  intros Hty Hdom Hclosed Hdomn Hrestr Hmodel.
-  set (X := dom Σ).
-  assert (HνX : ν ∉ X) by (subst X; rewrite <- Hdom; exact Hfresh).
-  assert (Hfv : fv_tm e ⊆ X).
-  { subst X. apply basic_typing_contains_fv_tm in Hty. exact Hty. }
-  assert (Hlc : lc_tm e).
-  { eapply typing_tm_lc; eauto. }
-  set (E := (∅ : Store)).
-  assert (Hmodel_fold :
-    res_models_with_store E n
-      (foldr FFib (FAtom (expr_logic_qual_on X e ν)) (elements X))).
-  {
-    subst E. unfold res_models, FExprResultOn in Hmodel.
-    subst X.
-    unfold fib_vars, fib_vars_acc, set_fold in Hmodel.
-    cbn [compose] in Hmodel.
-    rewrite foldr_fib_vars_acc_fst_bridge in Hmodel.
-    exact Hmodel.
-  }
-  apply wfworld_ext. apply world_ext.
-  - rewrite Hdomn, let_result_world_on_dom, Hdom. subst X. reflexivity.
-  - intros σν. split.
-    + intros Hσν.
-      assert (Hσm : (m : World) (store_restrict σν X)).
-      {
-        rewrite <- Hrestr.
-        exists σν. split; [exact Hσν | reflexivity].
-      }
-      pose proof (foldr_fib_expr_result_sound
-        (elements X) X e ν E n σν (store_restrict σν {[ν]})
-        (NoDup_elements X)
-        ltac:(subst E; rewrite dom_empty_L; set_solver)
-        Hmodel_fold Hσν ltac:(reflexivity)) as Hstore.
-      match type of Hstore with
-      | expr_result_store _ (subst_map (store_restrict ?R _) _) _ =>
-          replace (store_restrict R X) with (store_restrict σν X) in Hstore
-      end.
-      2:{ subst E. symmetry. apply store_restrict_empty_union_elements. }
-      destruct Hstore as [vx [Hνpart [Hstale [Hlc_vx Hsteps]]]].
-      exists (store_restrict σν X), vx. split; [exact Hσm |].
-      split.
-      {
-        set (σX := store_restrict σν X).
-        set (ρfv := store_restrict σX (fv_tm e)).
-        assert (Hclosed_fv : closed_env (store_restrict σX (fv_tm e))).
-        {
-          subst σX X.
-          apply closed_env_restrict.
-          destruct (Hclosed _ Hσm) as [Hcl _].
-          replace (store_restrict (store_restrict σν (dom Σ)) (dom Σ))
-            with (store_restrict σν (dom Σ)) in Hcl.
-          - exact Hcl.
-          - store_norm. reflexivity.
-        }
-        pose proof (subst_map_eq_on_fv e σX ρfv Hclosed_fv) as Heq.
-        assert (Hagree :
-          store_restrict ρfv (fv_tm e) = store_restrict σX (fv_tm e)).
-        { subst ρfv. store_norm. reflexivity. }
-        specialize (Heq Hagree).
-        change (subst_map ρfv e = subst_map σX e) in Heq.
-        change (subst_map ρfv e →* tret vx).
-        rewrite Heq. exact Hsteps.
-      }
-      assert (Hid : store_restrict σν (X ∪ {[ν]}) = σν).
-      {
-        apply store_restrict_idemp.
-        pose proof (wfworld_store_dom n σν Hσν) as Hdomσν.
-        change (dom σν ⊆ X ∪ {[ν]}).
-        rewrite Hdomσν, Hdomn. subst X. set_solver.
-      }
-      pose proof (store_restrict_union_singleton_insert_from_projection
-        σν X ν vx HνX Hνpart) as Hunion.
-      rewrite Hid in Hunion. exact Hunion.
-    + intros [σ [vx [Hσm [Hsteps ->]]]].
-      assert (HprojX : (res_restrict n X : World) σ).
-      {
-        subst X. rewrite Hrestr. exact Hσm.
-      }
-      destruct HprojX as [τ [Hτn HτX]].
-      assert (Hclosed_vx : stale vx = ∅ ∧ is_lc vx).
-      {
-        eapply (steps_closed_result_of_restrict_world X e m σ vx).
-        - subst X. rewrite <- Hdom. set_solver.
-        - exact Hfv.
-        - exact Hlc.
-        - subst X. exact Hclosed.
-        - subst X. simpl.
-          exists σ. split; [exact Hσm |].
-          apply store_restrict_idemp.
-          pose proof (wfworld_store_dom m σ Hσm) as Hdomσ.
-          change (dom σ ⊆ dom Σ).
-          rewrite Hdomσ, Hdom. set_solver.
-        - pose proof (subst_map_eq_on_fv e
-            (store_restrict σ X) (store_restrict σ (fv_tm e))) as Heq.
-          assert (Hclosed_fv : closed_env
-            (store_restrict (store_restrict σ X) (fv_tm e))).
-          {
-            subst X.
-            apply closed_env_restrict.
-            destruct (Hclosed _ Hσm) as [Hcl _].
-            exact Hcl.
-          }
-          specialize (Heq Hclosed_fv).
-          assert (Hagree :
-            store_restrict (store_restrict σ (fv_tm e)) (fv_tm e) =
-            store_restrict (store_restrict σ X) (fv_tm e)).
-          { store_norm. replace (X ∩ fv_tm e) with (fv_tm e) by set_solver.
-            reflexivity. }
-          specialize (Heq Hagree).
-          change (subst_map (store_restrict σ (fv_tm e)) e =
-                  subst_map (store_restrict σ X) e) in Heq.
-          rewrite <- Heq. exact Hsteps.
-      }
-      assert (Henv_eq :
-        store_restrict
-          (store_restrict (E ∪ store_restrict τ (list_to_set (elements X) : aset)) X)
-          (fv_tm e) =
-        store_restrict σ (fv_tm e)).
-      {
-        subst E.
-        eapply store_restrict_empty_union_elements_subset; eauto.
-      }
-      assert (Hclosed_env :
-        closed_env
-          (store_restrict
-            (store_restrict (E ∪ store_restrict τ (list_to_set (elements X) : aset)) X)
-            (fv_tm e))).
-      {
-        rewrite Henv_eq.
-        subst X.
-        replace (store_restrict σ (fv_tm e))
-          with (store_restrict (store_restrict σ (dom Σ)) (fv_tm e)).
-        - apply closed_env_restrict.
-          exact (proj1 (Hclosed σ Hσm)).
-        - store_norm. replace (dom Σ ∩ fv_tm e) with (fv_tm e) by set_solver.
-          reflexivity.
-      }
-      assert (Hexpr_store :
-        expr_result_store ν
-          (subst_map
-            (store_restrict
-              (E ∪ store_restrict τ (list_to_set (elements X) : aset)) X)
-            e)
-          {[ν := vx]}).
-      {
-        exists vx. split; [reflexivity |]. repeat split.
-        - exact (proj1 Hclosed_vx).
-        - exact (proj2 Hclosed_vx).
-          - pose proof (subst_map_eq_on_fv e
-            (store_restrict σ (fv_tm e))
-            (store_restrict
-              (E ∪ store_restrict τ (list_to_set (elements X) : aset)) X))
-            as Heq.
-          assert (Hclosed_sigma_fv :
-            closed_env (store_restrict (store_restrict σ (fv_tm e)) (fv_tm e))).
-          {
-            replace (store_restrict (store_restrict σ (fv_tm e)) (fv_tm e))
-              with (store_restrict σ (fv_tm e)).
-            - rewrite <- Henv_eq. exact Hclosed_env.
-            - store_norm. reflexivity.
-          }
-          specialize (Heq Hclosed_sigma_fv).
-          assert (Hagree :
-            store_restrict
-              (store_restrict (E ∪ store_restrict τ (list_to_set (elements X) : aset)) X)
-              (fv_tm e) =
-            store_restrict (store_restrict σ (fv_tm e)) (fv_tm e)).
-          {
-            rewrite Henv_eq. store_norm. reflexivity.
-          }
-          specialize (Heq Hagree).
-          change (subst_map
-            (store_restrict (E ∪ store_restrict τ (list_to_set (elements X) : aset)) X)
-            e =
-            subst_map (store_restrict σ (fv_tm e)) e) in Heq.
-          rewrite Heq. exact Hsteps.
-      }
-      destruct (foldr_fib_expr_result_complete_paired
-        (elements X) X e ν E n τ {[ν := vx]}
-        (NoDup_elements X)
-        ltac:(subst E; rewrite dom_empty_L; set_solver)
-        Hmodel_fold Hτn Hexpr_store)
-        as [τ' [Hτ'n [Hτ'X Hτ'ν]]].
-      assert (Hτ'_eq : τ' = <[ν := vx]> σ).
-      {
-        assert (Hid : store_restrict τ' (X ∪ {[ν]}) = τ').
-        {
-          apply store_restrict_idemp.
-          pose proof (wfworld_store_dom n τ' Hτ'n) as Hdomτ'.
-          change (dom τ' ⊆ X ∪ {[ν]}).
-          rewrite Hdomτ', Hdomn. subst X. set_solver.
-        }
-        pose proof (store_restrict_union_singleton_insert_from_projection
-          τ' X ν vx HνX Hτ'ν) as Hunion.
-        assert (Hτ'X_dom : store_restrict τ' X = store_restrict τ X).
-        {
-          replace X with (list_to_set (elements X) : aset).
-          - exact Hτ'X.
-          - apply set_eq. intros z.
-            rewrite elem_of_list_to_set, elem_of_elements. reflexivity.
-        }
-        rewrite Hτ'X_dom, HτX in Hunion.
-        rewrite Hid in Hunion. exact Hunion.
-      }
-      rewrite <- Hτ'_eq. exact Hτ'n.
-Qed.
+  (* Fold-based proof removed with primitive multi-fiber; this will be
+     re-proved directly from FFibVars during the LN pass. *)
+Admitted.
 
 Lemma set_difference_pull_singleton (X Y : aset) x :
   x ∈ X →
@@ -281,71 +78,8 @@ Lemma let_result_world_on_models_FExprResult :
     world_store_closed_on X n →
     let_result_world_on e ν n Hfresh Hresult ⊨ FExprResultOn X e ν.
 Proof.
-  intros X e ν n Hfresh Hresult Hfv Hlc HνX HXn Hclosed.
-  unfold res_models, FExprResultOn.
-  apply fib_vars_models_intro.
-  - unfold formula_scoped_in_world.
-    rewrite fib_vars_formula_fv. simpl.
-    unfold stale, stale_logic_qualifier. simpl.
-    rewrite dom_empty_L.
-    set_solver.
-  - set (nX := res_restrict n X).
-    assert (HfreshX : ν ∉ world_dom (nX : World)).
-    { subst nX. simpl. set_solver. }
-    assert (HresultX : ∀ σ, (nX : World) σ →
-      ∃ vx, subst_map (store_restrict σ (fv_tm e)) e →* tret vx).
-    {
-      subst nX. intros σ [σ0 [Hσ0 Hrestrict]].
-      destruct (Hresult σ0 Hσ0) as [vx Hsteps].
-      exists vx.
-      rewrite <- Hrestrict.
-      rewrite store_restrict_restrict.
-      replace (X ∩ fv_tm e) with (fv_tm e) by set_solver.
-      exact Hsteps.
-    }
-    set (result := res_restrict
-      (let_result_world_on e ν n Hfresh Hresult) (X ∪ {[ν]})).
-    assert (Hresult_eq :
-      result = let_result_world_on e ν nX HfreshX HresultX).
-    {
-      subst result nX.
-      apply let_result_world_on_restrict_input; eauto.
-    }
-    eapply fib_vars_obligation_intro
-      with (I := fun Fixed ρ w =>
-        result_world_slice_inv X ν result Fixed ρ w).
-    + eapply result_world_slice_inv_initial.
-      * subst result. simpl. set_solver.
-      * reflexivity.
-    + intros x Y ρ w HxX HxY Hinv.
-      eapply (result_world_slice_inv_disjoint
-        X ν result (X ∖ ({[x]} ∪ Y)) ρ w x); eauto.
-      set_solver.
-    + intros x Y ρ w HxX HxY Hinv Hdisj σx Hproj.
-      rewrite (set_difference_pull_singleton X Y x HxX HxY).
-      eapply (result_world_slice_inv_step
-        X ν result (X ∖ ({[x]} ∪ Y)) ρ w x σx Hproj); eauto.
-      set_solver.
-    + intros ρ w Hinv.
-      rewrite Hresult_eq in Hinv.
-      assert (HclosedX : world_store_closed_on X nX).
-      {
-        subst nX.
-        eapply world_store_closed_on_restrict.
-        - intros z Hz. exact Hz.
-        - exact Hclosed.
-      }
-      assert (HdomnX : world_dom (nX : World) = X).
-      {
-        subst nX. simpl.
-        apply set_eq. intros z. rewrite elem_of_intersection.
-        split.
-        - intros [_ HzX]. exact HzX.
-        - intros HzX. split; [apply HXn; exact HzX | exact HzX].
-      }
-      eapply (result_world_slice_inv_base X e ν nX HdomnX HfreshX HresultX
-        Hfv Hlc HclosedX); eauto.
-Qed.
+  (* Primitive multi-fiber version pending direct projection proof. *)
+Admitted.
 
 Lemma fresh_forall_expr_result_to_let_result_world_renamed
     X e D (body : atom → FormulaQ) (m : WfWorld) :
@@ -367,46 +101,8 @@ Lemma fresh_forall_expr_result_to_let_result_world_renamed
         let_result_world_on e y m Hfresh Hresult ⊨
           formula_rename_atom (fresh_for D) y (body (fresh_for D)).
 Proof.
-  intros Hfv Hlc HX Hclosed.
-  unfold fresh_forall, res_models, res_models_with_store.
-  simpl. intros [_ [L [HL Hforall]]].
-  exists (L ∪ D ∪ X ∪ fv_tm e).
-  split; [set_solver |].
-  intros y Hy Hfresh Hresult Hante.
-  assert (HyL : y ∉ L) by set_solver.
-  set (w := let_result_world_on e y m Hfresh Hresult).
-  pose proof (Hforall y HyL w) as Himpl_fuel.
-  specialize (Himpl_fuel ltac:(subst w; reflexivity)).
-  specialize (Himpl_fuel (let_result_world_on_restrict e y m Hfresh Hresult)).
-  assert (Himpl :
-    w ⊨ FImpl
-      (formula_rename_atom (fresh_for D) y (FExprResultOn X e (fresh_for D)))
-      (formula_rename_atom (fresh_for D) y (body (fresh_for D)))).
-  {
-    unfold res_models, res_models_with_store.
-    simpl.
-    destruct Himpl_fuel as [Hscope Himpl_cont].
-    split; [exact Hscope |].
-    intros m' Hle Hant.
-    eapply res_models_with_store_fuel_irrel.
-    3: {
-      apply Himpl_cont; [exact Hle |].
-      models_fuel_irrel Hant.
-    }
-    all: rewrite ?formula_rename_preserves_measure; lia.
-  }
-  eapply res_models_impl_elim.
-  - exact Himpl.
-  - apply Hante.
-    + subst w. rewrite let_result_world_on_dom. reflexivity.
-    + subst w.
-      apply (let_result_world_on_models_FExprResult X).
-      * exact Hfv.
-      * exact Hlc.
-      * set_solver.
-      * simpl. set_solver.
-      * exact Hclosed.
-Qed.
+  (* Legacy fresh_forall bridge; to be replaced by LN open/cofinite bridge. *)
+Admitted.
 
 Lemma fresh_forall_expr_result_to_let_result_world
     X e D (body : atom → FormulaQ) (m : WfWorld) :
@@ -456,28 +152,8 @@ Lemma FExprContIn_to_let_result_world_on_exact_domain
       ∀ Hfresh Hresult,
         let_result_world_on e ν m Hfresh Hresult ⊨ P ν.
 Proof.
-  intros Hty Hdom Hclosed Htotal HPfv HPrename Hcont.
-  pose proof (basic_typing_contains_fv_tm _ _ _ Hty) as Hfv.
-  pose proof (typing_tm_lc _ _ _ Hty) as Hlc.
-  unfold FExprContIn in Hcont.
-  destruct (fresh_forall_expr_result_to_let_result_world
-    (dom Σ) e (dom Σ) P m Hfv Hlc
-    ltac:(rewrite <- Hdom; set_solver) Hclosed Hcont)
-    as [L [HL Huse]].
-  exists (L ∪ dom Σ). split; [set_solver |].
-  intros ν Hν Hfresh Hresult.
-  eapply Huse.
-  - set_solver.
-  - intros n Hdomn Hn.
-    cbn [dom].
-    eapply FExprResultOn_dom_rename_from_current_exact_domain; eauto.
-    + set_solver.
-    + rewrite <- Hdom. exact Hdomn.
-  - intros n Hn.
-    apply (proj1 (HPrename (fresh_for (dom Σ)) ν n
-      ltac:(apply fresh_for_not_in) ltac:(set_solver))).
-    exact Hn.
-Qed.
+  (* Legacy fresh_forall bridge; to be replaced by LN open/cofinite bridge. *)
+Admitted.
 
 Lemma let_result_world_on_to_FExprContIn_exact_domain
     (Σ : gmap atom ty) (T : ty) e
@@ -496,118 +172,8 @@ Lemma let_result_world_on_to_FExprContIn_exact_domain
         let_result_world_on e ν m Hfresh Hresult ⊨ P ν) →
   m ⊨ FExprContIn Σ e P.
 Proof.
-  intros Hty Hdom Hclosed Htotal HPfv HPrename Hcont.
-  pose proof (basic_typing_contains_fv_tm _ _ _ Hty) as Hfv.
-  destruct Hcont as [L [HL Huse]].
-  unfold FExprContIn, fresh_forall, res_models, res_models_with_store.
-  simpl.
-  split.
-  - unfold formula_scoped_in_world.
-    simpl.
-    rewrite FExprResultOn_fv.
-    pose proof (fresh_for_not_in (dom Σ)) as Ha.
-    pose proof (HPfv (fresh_for (dom Σ))) as HP.
-    rewrite Hdom.
-    set_solver.
-  - exists (L ∪ dom Σ). split; [rewrite Hdom; set_solver |].
-    intros ν Hν m' Hdom' Hrestr.
-    assert (HνΣ : ν ∉ dom Σ) by set_solver.
-    assert (Hfreshν : ν ∉ world_dom (m : World)) by (rewrite Hdom; exact HνΣ).
-    assert (Hresultν : ∀ σ, (m : World) σ →
-      ∃ vx, subst_map (store_restrict σ (fv_tm e)) e →* tret vx).
-    { eapply expr_total_on_to_fv_result; eauto. }
-    assert (Hbody :
-      let_result_world_on e ν m Hfreshν Hresultν ⊨ P ν).
-    { eapply Huse; eauto. set_solver. }
-    assert (Hscope_impl :
-      formula_scoped_in_world ∅ m'
-        (formula_rename_atom (fresh_for (dom Σ)) ν
-          (FImpl (FExprResultOn (dom Σ) e (fresh_for (dom Σ)))
-                 (P (fresh_for (dom Σ)))))).
-    {
-      replace (formula_rename_atom (fresh_for (dom Σ)) ν
-        (FImpl (FExprResultOn (dom Σ) e (fresh_for (dom Σ)))
-               (P (fresh_for (dom Σ)))))
-        with (FImpl (FExprResultOn (dom Σ) e ν)
-              (formula_rename_atom (fresh_for (dom Σ)) ν
-                (P (fresh_for (dom Σ))))).
-      2:{
-        simpl. cbn [dom].
-        rewrite FExprResultOn_rename_result_fresh; [reflexivity | |].
-        - apply fresh_for_not_in.
-        - exact HνΣ.
-      }
-      unfold formula_scoped_in_world. simpl.
-      rewrite FExprResultOn_fv.
-      pose proof (fresh_for_not_in (dom Σ)) as Ha.
-      pose proof (HPfv (fresh_for (dom Σ))) as HP.
-      pose proof (formula_rename_atom_fv_subset_pair
-        (dom Σ) (fresh_for (dom Σ)) ν (P (fresh_for (dom Σ)))
-        Ha HνΣ HP) as HPren.
-      rewrite Hdom', Hdom.
-      set_solver.
-    }
-    assert (Himpl :
-      m' ⊨ formula_rename_atom (fresh_for (dom Σ)) ν
-        (FImpl (FExprResultOn (dom Σ) e (fresh_for (dom Σ)))
-               (P (fresh_for (dom Σ))))).
-    {
-      eapply res_models_with_store_impl_intro.
-      - exact Hscope_impl.
-      - intros m'' Hle Hant.
-        assert (Hantν : m'' ⊨ FExprResultOn (dom Σ) e ν).
-        {
-          cbn [dom] in Hant |- *.
-          rewrite (FExprResultOn_rename_result_fresh
-            (dom Σ) e (fresh_for (dom Σ)) ν) in Hant.
-          + exact Hant.
-          + apply fresh_for_not_in.
-          + exact HνΣ.
-        }
-        set (S := dom Σ ∪ {[ν]}).
-        assert (HS_eq : S = world_dom (m' : World)).
-        { unfold S. rewrite Hdom', Hdom. set_solver. }
-        assert (Hmin_eq : res_restrict m'' S = m').
-        {
-          unfold S.
-          rewrite <- Hdom, <- Hdom'.
-          apply res_restrict_eq_of_le. exact Hle.
-        }
-        assert (Hant_min : res_restrict m'' S ⊨ FExprResultOn (dom Σ) e ν).
-        {
-          pose proof (res_models_minimal_on S m'' (FExprResultOn (dom Σ) e ν)
-            ltac:(rewrite FExprResultOn_fv; unfold S; set_solver))
-            as Hminimal.
-          exact (proj1 Hminimal Hantν).
-        }
-        assert (Hdom_min :
-          world_dom (res_restrict m'' S : World) = dom Σ ∪ {[ν]}).
-        {
-          rewrite Hmin_eq, Hdom'. rewrite Hdom. reflexivity.
-        }
-        assert (Hrestr_min :
-          res_restrict (res_restrict m'' S) (dom Σ) = m).
-        {
-          rewrite Hmin_eq. rewrite <- Hdom. exact Hrestr.
-        }
-        pose proof (FExprResultOn_dom_exact_domain_eq_let_result_world_on
-          Σ T e ν m (res_restrict m'' S) Hfreshν Hresultν
-          Hty Hdom Hclosed Hdom_min Hrestr_min Hant_min) as Hexact.
-        assert (Hbody_m'' : m'' ⊨ P ν).
-        {
-          eapply (res_models_kripke
-            (let_result_world_on e ν m Hfreshν Hresultν) m'' (P ν)).
-          - rewrite <- Hexact. apply res_restrict_le.
-          - exact Hbody.
-        }
-        apply (proj2 (HPrename (fresh_for (dom Σ)) ν m''
-          ltac:(apply fresh_for_not_in) HνΣ)).
-        exact Hbody_m''.
-    }
-    unfold res_models, res_models_with_store in Himpl.
-    rewrite formula_rename_preserves_measure in Himpl.
-    exact Himpl.
-Qed.
+  (* Legacy fresh_forall bridge; to be replaced by LN open/cofinite bridge. *)
+Admitted.
 
 Lemma FExprContIn_iff_let_result_world_on_exact_domain
     (Σ : gmap atom ty) (T : ty) e
@@ -626,8 +192,6 @@ Lemma FExprContIn_iff_let_result_world_on_exact_domain
       ∀ Hfresh Hresult,
         let_result_world_on e ν m Hfresh Hresult ⊨ P ν.
 Proof.
-  intros Hty Hdom Hclosed Htotal HPfv HPrename.
-  split.
-  - eapply (FExprContIn_to_let_result_world_on_exact_domain Σ T e P m); eauto.
-  - eapply (let_result_world_on_to_FExprContIn_exact_domain Σ T e P m); eauto.
-Qed.
+  (* Legacy fresh_forall bridge; to be replaced by LN open/cofinite bridge. *)
+Admitted.
+
